Addressed PR feedback

isabelle/Util/Division.thy
@@ -13,8 +13,8 @@ fun quot :: "int \<Rightarrow> int \<Rightarrow> int" (infixl "quot" 70) where
 "x quot y = (if (x < 0) = (y < 0) then x div y else -(abs x div abs y))"
 
 
-text \<open>With the \<^emph>\<open>div\<close> operator, if the numerator is lower than the denominator 
-(in absolute), then the division is rounded to \<^term>\<open>-1\<close>. With the \<^emph>\<open>quot\<close> 
+text \<open>With the \<^emph>\<open>div\<close> operator, if the numerator is lower than the denominator
+(in absolute), then the division is rounded to \<^term>\<open>-1\<close>. With the \<^emph>\<open>quot\<close>
 operator that division is rounded to zero. For example:\<close>
 proposition "2 div -3  = (-1 :: int)"
             "-2 div 3  = (-1 :: int)"
@@ -22,18 +22,16 @@ proposition "2 div -3  = (-1 :: int)"
             "-2 quot 3 = 0"
   by simp_all
 
-text "More generally" 
+text "More generally"
 
-lemma quot_rounds_to_zero : 
-  assumes "\<bar>n\<bar> < \<bar>d\<bar>" 
-    shows "n quot d = 0" 
+lemma quot_rounds_to_zero :
+  assumes "\<bar>n\<bar> < \<bar>d\<bar>"
+    shows "n quot d = 0"
   using assms by auto
 
 
 lemma quot_by_zero_is_zero : "n quot 0 = 0"
   by auto
-
-
 
 lemma quotMultiplyEquivalence : "c \<noteq> 0 \<Longrightarrow> (c * a) quot (c * b) = a quot b"
   apply auto
@@ -42,4 +40,74 @@ lemma quotMultiplyEquivalence : "c \<noteq> 0 \<Longrightarrow> (c * a) quot (c 
   apply (smt div_minus_minus mult_minus_right nonzero_mult_div_cancel_left zdiv_zmult2_eq)
   apply (metis div_minus_right div_mult_mult1 mult_minus_right)
   by (metis div_mult_mult1 less_irrefl mult_minus_right)
+
+section "Unused"
+
+text \<open>The following functions and lemmas are not used by the rest of the theories.\<close>
+
+fun signum :: "int \<Rightarrow> int" where
+"signum x = (if x > 0 then 1 else if x = 0 then 0 else -1)"
+
+fun rem :: "int \<Rightarrow> int \<Rightarrow> int" (infixl "rem" 70) where
+"x rem y = x - (x quot y) * y"
+
+fun quotRem :: "int \<Rightarrow> int \<Rightarrow> int \<times> int" (infixl "quotRem" 70) where
+"x quotRem y = (x quot y, x rem y)"
+
+lemma remMultiplyEquivalence : "c \<noteq> 0 \<Longrightarrow> (c * a) rem (c * b) = c * (a rem b)"
+proof -
+  assume "c \<noteq> 0"
+  then have "\<And>i ia. c * i quot (c * ia) = i quot ia"
+    using quotMultiplyEquivalence by presburger
+  then show ?thesis
+    by (simp add: right_diff_distrib')
+qed
+
+lemma signEqualityPreservation : "(a :: int) \<noteq> 0 \<Longrightarrow> (b :: int) \<noteq> 0 \<Longrightarrow> (c :: int) \<noteq> 0 \<Longrightarrow> ((c * a < 0) = (c * b < 0)) = ((a < 0) = (b < 0))"
+  by (smt mult_neg_pos mult_nonneg_nonneg mult_nonpos_nonpos mult_pos_neg)
+
+lemma divMultiply : "(c :: int) \<noteq> 0 \<Longrightarrow> (c * a) div (c * b) = a div b"
+  by simp
+lemma divAbsMultiply : "(c :: int) \<noteq> 0 \<Longrightarrow> \<bar>c * a\<bar> div \<bar>c * b\<bar> = \<bar>a\<bar> div \<bar>b\<bar>"
+  by (simp add: abs_mult)
+
+lemma addMultiply : "\<bar>(c :: int) * a + x * (c * b)\<bar> = \<bar>c * (a + x * b)\<bar>"
+  by (simp add: distrib_left mult.left_commute)
+
+lemma addAbsMultiply : "\<bar>(c :: int) * a + x * (c * b)\<bar> = \<bar>c * (a + x * b)\<bar>"
+  by (simp add: distrib_left mult.left_commute)
+
+lemma subMultiply : "\<bar>(c :: int) * a - x * (c * b)\<bar> = \<bar>c * (a - x * b)\<bar>"
+  by (simp add: mult.left_commute right_diff_distrib')
+
+lemma ltMultiply : "(c :: int) \<noteq> 0 \<Longrightarrow> (\<bar>x\<bar> * 2 < \<bar>b\<bar>) = (\<bar>c * x\<bar> * 2 < \<bar>c * b\<bar>)"
+  by (simp add: abs_mult)
+
+lemma remMultiplySmalle_aux : "(a :: int) \<noteq> 0 \<Longrightarrow> (b :: int) \<noteq> 0 \<Longrightarrow> (c :: int) \<noteq> 0 \<Longrightarrow> (\<bar>a - a div b * b\<bar> * 2 < \<bar>b\<bar>) = (\<bar>c * a - c * a div (c * b) * (c * b)\<bar> * 2 < \<bar>c * b\<bar>)"
+  apply (subst divMultiply)
+  apply simp
+  apply (subst subMultiply)
+  using ltMultiply by blast
+
+lemma remMultiplySmalle_aux2 : "(a :: int) \<noteq> 0 \<Longrightarrow> (b :: int) \<noteq> 0 \<Longrightarrow> (c :: int) \<noteq> 0 \<Longrightarrow> (\<bar>a + \<bar>a\<bar> div \<bar>b\<bar> * b\<bar> * 2 < \<bar>b\<bar>) = (\<bar>c * a + \<bar>c * a\<bar> div \<bar>c * b\<bar> * (c * b)\<bar> * 2 < \<bar>c * b\<bar>)"
+  apply (subst divAbsMultiply)
+  apply simp
+  apply (subst addMultiply)
+  using ltMultiply by blast
+
+lemma remMultiplySmaller : "c \<noteq> 0 \<Longrightarrow> (\<bar>a rem b\<bar> * 2 < \<bar>b\<bar>) = (\<bar>(c * a) rem (c * b)\<bar> * 2 < \<bar>c * b\<bar>)"
+  apply (cases "b = 0")
+  apply simp
+  apply (cases "a = 0")
+  apply (simp add: mult_less_0_iff)
+  apply (simp only:quot.simps rem.simps)
+  apply (subst signEqualityPreservation[of a b c])
+  apply simp
+  apply simp
+  apply simp
+  apply (cases "(a < 0) = (b < 0)")
+  apply (simp only:if_True refl)
+  using remMultiplySmalle_aux apply blast
+  apply (simp only:if_False refl)
+  by (metis (no_types, opaque_lifting) diff_minus_eq_add mult_minus_left remMultiplySmalle_aux2)
 end
